@prefix : <https://w3id.org/won/ext/hold#> .
@prefix owl: <http://www.w3.org/2002/07/owl#> .
@prefix rdf: <http://www.w3.org/1999/02/22-rdf-syntax-ns#> .
@prefix won: <https://w3id.org/won/core#> .
@prefix xml: <http://www.w3.org/XML/1998/namespace> .
@prefix xsd: <http://www.w3.org/2001/XMLSchema#> .
@prefix rdfs: <http://www.w3.org/2000/01/rdf-schema#> .
@base <https://w3id.org/won/ext/hold> .

<https://w3id.org/won/ext/hold> rdf:type owl:Ontology ;
                                 owl:imports <https://w3id.org/won/core> .

#################################################################
#    Object Properties
#################################################################

###  https://w3id.org/won/ext/hold#heldBy
:heldBy rdf:type owl:ObjectProperty ;
        owl:inverseOf :holds ;
        rdfs:domain won:Atom ;
        rdfs:range won:Atom .


###  https://w3id.org/won/ext/hold#holds
:holds rdf:type owl:ObjectProperty ;
       rdfs:domain won:Atom ,
                   :Holder ;
       rdfs:range won:Atom ,
                  :Holdable .


#################################################################
#    Classes
#################################################################


###  https://w3id.org/won/ext/hold#Holdable
:Holdable rdf:type owl:Class ;
          rdfs:comment "An Atom that does not represent an agent. May be connected to a Holder Atom via the heldBy property."@en .


###  https://w3id.org/won/ext/hold#Holder
:Holder rdf:type owl:Class ;
        rdfs:comment "Represents an agent. Is linked to other Atoms the agent controls via the holds property."@en .


#################################################################
#    Individuals
#################################################################


###  https://w3id.org/won/ext/hold#HoldableSocket
:HoldableSocket rdf:type owl:NamedIndividual ,
                         won:Socket ;
                won:allowedTargetSocket :HolderSocket ;
                won:derivesAtomProperty :holds ;
                won:overloadPolicy won:OnOverloadDeny ;
                won:autoOpen "false"^^xsd:boolean ;
                won:socketCapacity 1 ;
                rdfs:comment "An Atom uses this Socket to connect to the Persona Atom that holds it."@en .


###  https://w3id.org/won/ext/hold#HolderSocket
:HolderSocket rdf:type owl:NamedIndividual ,
                       won:Socket ;
              won:allowedTargetSocket :HoldableSocket ;
              won:derivesAtomProperty :heldBy ;
              won:autoOpen "false"^^xsd:boolean ;
              rdfs:comment "A Persona Atom uses this Socket to connect to Atoms it holds."@en .


###  https://w3id.org/won/ext/hold#heldBy
:heldBy rdf:type owl:NamedIndividual .


###  https://w3id.org/won/ext/hold#holds
:holds rdf:type owl:NamedIndividual .


#################################################################
#    Annotations
#################################################################

:heldBy rdfs:comment "Links an Atom to the Atom representing the agent (a person, organization, bot, ...) that controls both."@en .


:holds rdfs:comment "Links the Atom representing an agent (a person, organization, bot, ...) to another Atom they control."@en .


###  Generated by the OWL API (version 4.2.8.20170104-2310) https://github.com/owlcs/owlapi
